@prefix : <http://voc.orchestracities.io/oc-acl#> .
@prefix dc: <http://purl.org/dc/elements/1.1/> .
@prefix acl: <http://www.w3.org/ns/auth/acl#> .
@prefix rdf: <http://www.w3.org/1999/02/22-rdf-syntax-ns#> .
@prefix xml: <http://www.w3.org/XML/1998/namespace> .
@prefix xsd: <http://www.w3.org/2001/XMLSchema#> .
@prefix foaf: <http://xmlns.com/foaf/0.1/> .
@prefix odrl: <http://www.w3.org/ns/odrl/2/> .
@prefix rdfs: <http://www.w3.org/2000/01/rdf-schema#> .
@prefix owl: <http://www.w3.org/2002/07/owl#> .
@base <http://voc.orchestracities.io/oc-acl#> .

<>
  dc:title "Anubis Access Control vocabulary" ;
  rdfs:comment "Extend W3C Web Access Control with custom definitions for Anubis. " ;
  rdfs:seeAlso "https://anubis-pep.readthedocs.io/en/latest/" .


#################################################################
#    Object Properties
#################################################################

###  http://voc.orchestracities.io/oc-acl#constraint
:constraint a rdf:Property , owl:ObjectProperty ;
            rdfs:domain acl:Authorization ;
            rdfs:range [ a owl:Class ;
                         owl:unionOf ( odrl:Constraint
                                       odrl:LogicalConstraint
                                     )
                       ] ;
            rdfs:comment "The rules to be satisfied to access the resource" ;
            rdfs:label "Has Constraint"@en .


###  http://voc.orchestracities.io/oc-acl#attributeName
:attributeName a rdf:Property , owl:ObjectProperty ;
            rdfs:domain :GenericLeftOperand ;
            rdfs:range rdfs:Literal ;
            rdfs:comment "The name of the attribute to which the operand is applied" ;
            rdfs:label "Has Attribute Name"@en .

###  http://voc.orchestracities.io/oc-acl#scope
:scope a rdf:Property , owl:ObjectProperty ;
            rdfs:domain :GenericLeftOperand ;
            rdfs:range :Scope ;
            rdfs:comment "The scope of the operand (object or subject)" ;
            rdfs:label "Has scope"@en .

#################################################################
#    Classes
#################################################################

###  http://voc.orchestracities.io/oc-acl#Delete
:Delete a rdfs:Class ;
        rdfs:subClassOf acl:Access ,
                        acl:Write ;
        rdfs:comment "Delete accesses are specific write access which only delete information." ;
        rdfs:label "Delete"@en .


###  http://voc.orchestracities.io/oc-acl#ResourceTenantAgent
:ResourceTenantAgent a rdfs:Class ;
                     rdfs:subClassOf acl:AuthenticatedAgent ,
                                     foaf:Agent ;
                     rdfs:comment """A class of agents who have been authenticated and that belongs
to the same Tenant to which the resource requested belongs.
In other words, anyone who belong to the same Tenant as the resource can access
this resource, but not anonymously.
""" ;
                     rdfs:label "Resource Tenant Agent"@en .


###  http://voc.orchestracities.io/oc-acl#GenericLeftOperand
:GenericLeftOperand a rdfs:Class , owl:Class ;
                    rdfs:subClassOf odrl:LeftOperand ;
                    rdfs:comment """A left operand that allows to define the scope
of the operand, and the attribute to which the operand apply
""" ;
                    rdfs:label "Generic Left Operand"@en .


###  http://voc.orchestracities.io/oc-acl#Scope
:Scope a rdfs:Class , owl:Class ;
                    rdfs:comment """The scope of a left operand""" ;
                    rdfs:label "Scope"@en .


#################################################################
#    Individuals
#################################################################

###  http://voc.orchestracities.io/oc-acl#subject
:subject a owl:NamedIndividual , :Scope ;
  rdfs:label "Subject"@en .

###  http://voc.orchestracities.io/oc-acl#object
:object a owl:NamedIndividual , :Scope ;
  rdfs:label "Object"@en .


#################################################################
#    Annotations
#################################################################

<https://anubis-pep.readthedocs.org/> dc:describes <> .


<https://github.com/orchestracities/anubis-vocabulary> dc:describes <> .


###  Generated by the OWL API (version 4.5.9.2019-02-01T07:24:44Z) https://github.com/owlcs/owlapi
