@prefix : <http://voc.orchestracities.io/oc-acl#> .
@prefix dc: <http://purl.org/dc/elements/1.1/> .
@prefix acl: <http://www.w3.org/ns/auth/acl#> .
@prefix rdf: <http://www.w3.org/1999/02/22-rdf-syntax-ns#> .
@prefix xml: <http://www.w3.org/XML/1998/namespace> .
@prefix xsd: <http://www.w3.org/2001/XMLSchema#> .
@prefix foaf: <http://xmlns.com/foaf/0.1/> .
@prefix odrl: <http://www.w3.org/ns/odrl/2/> .
@prefix rdfs: <http://www.w3.org/2000/01/rdf-schema#> .
@prefix owl: <http://www.w3.org/2002/07/owl#> 
@base <http://voc.orchestracities.io/oc-acl#> .

<>
  dc:title "Anubis Access Control vocabulary" ;
  rdfs:comment "Extend W3C Web Access Control with custom definitions for Anubis. " ;
  rdfs:seeAlso "https://anubis-pep.readthedocs.io/en/latest/" .


#################################################################
#    Object Properties
#################################################################

###  http://voc.orchestracities.io/oc-acl#constraint
:constraint a rdf:Property , owl:ObjectProperty ;
            rdfs:domain acl:Authorization ;
            rdfs:range [ a owl:Class ;
                         owl:unionOf ( odrl:Constraint
                                       odrl:LogicalConstraint
                                     )
                       ] ;
            rdfs:comment "The rules to be satisfied to access the resource" ;
            rdfs:label "Has Constraint"@en .


#################################################################
#    Classes
#################################################################

###  http://voc.orchestracities.io/oc-acl#Delete
:Delete a rdfs:Class ;
        rdfs:subClassOf acl:Access ,
                        acl:Write ;
        rdfs:comment "Delete accesses are specific write access which only delete information." ;
        rdfs:label "Delete"@en .


###  http://voc.orchestracities.io/oc-acl#ResourceTenantAgent
:ResourceTenantAgent a rdfs:Class ;
                     rdfs:subClassOf acl:AuthenticatedAgent ,
                                     foaf:Agent ;
                     rdfs:comment """A class of agents who have been authenticated and that belongs
to the same Tenant to which the resource requested belongs.
In other words, anyone who belong to the same Tenant as the resource can access
this resource, but not anonymously.
""" ;
                     rdfs:label "Resource Tenant Agent"@en .

#################################################################
#    Annotations
#################################################################

<https://anubis-pep.readthedocs.org/> dc:describes <> .


<https://github.com/orchestracities/anubis-vocabulary> dc:describes <> .


###  Generated by the OWL API (version 4.5.9.2019-02-01T07:24:44Z) https://github.com/owlcs/owlapi
